filling out LSN-based journal spec

Splinter/Journal.i.dfy
@@ -3,6 +3,7 @@ include "../lib/Base/Maps.i.dfy"
 include "Spec.s.dfy"
 include "MsgSeq.i.dfy"
 include "Tables.i.dfy"
+include "CacheIfc.i.dfy"
 
 
 // NB the journal needs a smaller-sized-write primitive. If we get asked to sync
@@ -18,11 +19,13 @@ module JournalMachineMod {
   import opened MsgSeqMod
   import opened AllocationMod
   import AllocationTableMod
+  import CacheIfc
+  import MarshalledSnapshot // TODO stub delete
 
   // The core journal superblock
   datatype CoreSuperblock = CoreSuperblock(
     freshestCU: Option<CU>,
-    firstValidLSN : LSN)
+    boundaryLSN : LSN)
 
   // The entire superblock we need to store: Core data plus allocation data
   datatype Superblock = Superblock(
@@ -36,7 +39,7 @@ module JournalMachineMod {
   )
 
   datatype Variables = Variables(
-    firstValidLSN: LSN,
+    boundaryLSN: LSN,
       // The (exclusive) upper bound of LSNs reachable from the
       // last-known-committed superblock; earlier LSNs have already been
       // garbage-collected. (There may be leftover records with smaller LSNs in
@@ -49,82 +52,88 @@ module JournalMachineMod {
       // We may need to track this value to ensure commit doesn't go backwards.
       // (maybe invariant-able)
 
-    durableLSN: LSN,
-      // The (exclusive) upper bound of LSNs that could be made persistent with a
-      // superblock write. (They're covered by marshalled pages that have been written
-      // back to the disk, but aren't yet linked to the superblock.)
+    cleanLSN: LSN,
+      // The (exclusive) upper bound of LSNs that could be made persistent with
+      // a superblock write. They're covered by marshalled pages that are
+      // "clean" (have been written back to the disk), but aren't yet linked to
+      // the superblock. These pages aren't "durable" or "persistent", because if there
+      // were a crash right now, they'd be unallocated garbage after the crash.
 
     marshalledLSN: LSN,
-      // The (exclusive) upper bound
+      // The (exclusive) upper bound of LSNs that have been marshalled into cache
+      // blocks.
 
-    durableTailCU: Option<CU>,
-      // pointer to the freshest CU that's durable (okay to commit in SB)
+    unmarshalledTail: seq<Message>,
+      // The rest of the in-memory journal
 
-    seqStart: LSN,  // in-memory records start here
-    journal: seq<MemJournalRecord>, // in memory records
-    seqToAU: map<LSN, AU>,  // Which AU each seq number is stored in.
-    syncReqs: map<SyncReqId, LSN>
+    syncReqs: map<SyncReqId, LSN>,
+      // The LSN each outstanding SyncRequest was created at. The sync request may be
+      // completed when the corresponding LSN <= persistentLSN.
+
+    lsnToCU: map<LSN, CU>
+      // We imagine that the journal can keep track of the entire mapping from LSN to CUs.
+      // That's not really how the impl will work; it'll maintain some sort of summary, and
+      // we'll refine from the disk state to get this field.
   )
   {
-    predicate seqToAuValid() {
-      && forall seqno :: firstValidLSN <= seqno < seqStart <==> seqno in seqToAU.Keys
+    // The (exclusive) upper bound of LSNs that have been journaled (in this epoch;
+    // after a crash we can lose LSNs that weren't made persistent).
+    function unmarshalledLSN() : LSN
+    {
+      marshalledLSN + |unmarshalledTail|
     }
 
     predicate WF() {
-      && seqToAuValid()
+      && boundaryLSN <= persistentLSN <= cleanLSN <= marshalledLSN
+      && (forall lsn :: 0 <= lsn < unmarshalledLSN() <==> lsn in lsnToCU)
     }
   }
-
-//////////////////////////////////////////////////////////////////////////////
-/*
-Journal operations include:
-- Append(Message): find the open CU and concat the message (cache write)
-- Advance(): the open CU is full. Open a new one with a back-pointer. (cache write)
-  Depends on being able to identify an unutilized CU, which requires knowing which CUs
-  in the disk journal are allocated.
-- Reallocate(): allocate or free AUs
-- CommitStart(sb): sb becomes eligible to be the next superblock
-  - PagesAreClean(lastCUexcl): the pages for CUs from sb.freshestCU to lastCUexcl are clean
-    (what to do when sb.freshestCU is None?
-- CommitComplete(sb): sb is definitely the next superblock
-- Replay(): needed at recovery time
-
-A completely empty journal has firstCU.None?, firstValidLSN==0
-A fully-garbage-collected journal has firstCU.None?, firstValidLSN positive
-
-Invariants:
-- I think we need a ghost relation between journal cus and LSNs
-- Only pages "between" durableCU and tailCU are dirty in cache
-
-*/
 
   // advances tailLSN forward by adding a message
   predicate Append(s: Variables, s': Variables, message: Message)
   {
-    && s' == s.(openRecord := s.openRecord.Extend(message))
+    && s' == s.(unmarshalledTail := s.unmarshalledTail + [message])
+  }
+
+  function AllocateEmptyCU(s: Variables) : CU
+  {
+    CU(0, 0) //TODO
+  }
+
+    // TODO marshalling
+  function parse(b: UninterpretedDiskPage) : Option<JournalRecord>
+  function marshal(jr: JournalRecord) : UninterpretedDiskPage
+
+  function TailToMsgSeq(s: Variables) : MsgSeq
+  {
+    var start := s.marshalledLSN;
+    var end := start + |s.unmarshalledTail|;
+    MsgSeq(map i:LSN | start <= i < end :: s.unmarshalledTail[i - start], start, end)
   }
 
   // advances marshalledLSN forward by marshalling a batch of messages into a dirty cache page
-  predicate AdvanceMarshalled(s: Variables, s': Variables, cop: CacheIfc.Ops)
+  predicate AdvanceMarshalled(s: Variables, s': Variables, cacheOps: CacheIfc.Ops)
   {
+    && s.WF()
     && var cu := AllocateEmptyCU(s);
     // Marshal and write the current record out into the cache. (This doesn't issue
     // a disk write, it just dirties a page.)
-    && var jr := JournalRecord(s.openRecord, s.tailCU)
-    && cop == [CacheIfc.Write(cu, marshal(jr))]
+    && var priorLSN := if s.marshalledLSN==0 then None else Some(s.lsnToCU[s.marshalledLSN-1]);
+    && var jr := JournalRecord(TailToMsgSeq(s), priorLSN);
+    && cacheOps == [CacheIfc.Write(cu, marshal(jr))]
     && s' == s.(
       // Open a new, empty record to absorb future journal Appends
-      openRecord := MsgSeq([], s.openRecord.seqEnd, s.openRecord.seqEnd)
-      seqToAU := MergeAu(s.seqToAU, cu.au, s.openRecord))
+      unmarshalledTail := [])
   }
 
-  // advances durableLSN forward by learning that the cache has written back a contiguous
-  // sequence of pages starting at last durableCU
-  predicate AdvanceDurable(s: Variables, s': Variables, int k, cache: CacheIfc.Variables)
+  // advances cleanLSN forward by learning that the cache has written back a contiguous
+  // sequence of pages starting at last cleanLSN
+  predicate AdvanceClean(s: Variables, s': Variables, cache: CacheIfc.Variables, newClean: nat)
   {
-    && var jc := JournalChain(marshalledCU, durableCU, cache);
-    && (forall i | 0<i<k :: cache.IsClean(jc[i]))
-    && s' == s.(durableCU := jc[k])
+    && s.WF()
+    && s.cleanLSN < newClean <= s.marshalledLSN
+    && (forall lsn | s.cleanLSN <= lsn < newClean :: && CacheIfc.IsClean(cache, s.lsnToCU[lsn]))
+    && s' == s.(cleanLSN := newClean)
   }
 
   predicate Reallocate(s: Variables, s': Variables)
@@ -134,25 +143,26 @@ Invariants:
 
   function ParseCachedRecord(cache: CacheIfc.Variables, cu: CU) : Option<JournalRecord>
   {
-    var raw := CacheIfc.ReadValue(s, cu);
+    var raw := CacheIfc.ReadValue(cache, cu);
     if raw.Some? then parse(raw.value) else None
   }
 
-  // Agrees to advance persistentLSN (to durableLSN) and firstLSN (to newBoundary, coordinated
+  // Agrees to advance persistentLSN (to cleanLSN) and firstLSN (to newBoundary, coordinated
   // with BeTree) as part of superblock writeback.
-  predicate CommitStart(s: Variables, s': Variables, cache: CacheIfc.Variables, sb: Superblock, newBoundary: LSN)
+  predicate CommitStart(s: Variables, s': Variables, cache: CacheIfc.Variables, sb: Superblock, newBoundaryLSN: LSN)
   {
-    // Boundary advances from oldBoundary to newBoundary (maybe zero)
-    && var oldBoundary := s.firstValidLSN;
-    && oldBoundary <= newBoundary // presumably provable from Inv
+    && s.WF()
+    // This is the stuff we'll get to garbage collect when the sb commit completes.
+    && s.boundaryLSN <= newBoundaryLSN // presumably provable from Inv
 
-    // Persistent advances from oldPersistent to durableLSN
-    && var oldPersistent := /*s.persistentTailLSN computable from cur sb*/;
-    && var newPersistent := s.durableLSN; // TODO compute from durableCU and LSN<->cu relation?
-    && oldPersistent <= newPersistent;
+    // These are the LSNs whose syncs will complete when the sb commit completes.
+    && s.persistentLSN <= s.cleanLSN  // presumably provable from Inv
 
-    //
-    && sb == Superblock(CoreSuperblock(s.durableTailCU, newBoundary), allocationInfo)
+    // This is the superblock that's going to become persistent.
+    && var allocationInfo := AllocationTableMod.Superblock(AllocationTableMod.SnapshotSuperblock(CU(0, 0))); // TODO
+    && var freshestCU := if s.cleanLSN == 0 then None else Some(s.lsnToCU[s.cleanLSN-1]);
+    && sb == Superblock(allocationInfo, CoreSuperblock(freshestCU, newBoundaryLSN))
+      // TODO what f s.cleanLSN is zero or ... no priorCU?
     && s' == s
   }
 
@@ -160,365 +170,63 @@ Invariants:
   predicate CommitComplete(s: Variables, s': Variables, sb: Superblock)
   {
     && s.WF()
-    && s'.firstValidLSN == sb.core.firstValidLSN  // bump the boundary forward now.
-    && s'.durableTailCU == s.durableTailCU
-    && s'.seqStart == s.seqStart
-    && s'.journal == s.journal
-    && s'.seqToAU == (map seqno | s'.firstValidLSN <= seqno < s'.seqStart :: s.seqToAU[seqno])
-    && s'.syncReqs == s.syncReqs
-  }
 
+    && s'.boundaryLSN == sb.core.boundaryLSN
 
-//////////////////////////////////////////////////////////////////////////////
-
-  predicate SeqsCoveredByAllocation(s:Variables, seqStart: LSN, seqEndExclusive: LSN, allocation: AllocationTableMod.Superblock)
-  {
-    false
-  }
-
-  predicate Record(s: Variables, s': Variables, message: Message)
-  {
-    && s' == s.(journal := s.journal + [Message(message)])
-  }
-
-  predicate InitiateJournalWriteNoop(s: Variables, s': Variables)
-  {
-    false
-  }
-
-  predicate CompleteJournalWriteNoop(s: Variables, s': Variables)
-  {
-    false
-  }
-
-  predicate InitiateSuperblockWriteNoop(s: Variables, s': Variables)
-  {
-    false
-  }
-
-  predicate AsyncFlush(s: Variables, s': Variables)
-  {
-    false
-    // Complete superblock write
-    // a superblock write hits the disk and commits seqStart .. seqStart + inFlightWriteCount
-  }
-
-  function endLSNExclusive(firstValidLSN: LSN, cu: Option<CU>) : LSN
-  {
-    0 //TODO
-  }
-
-  // Program keeps track of the "in-flight" superblock. CommitStart(sb) means that sb
-  // is being sent to disk, and CommitComplete(sb) is confirmation that sb is now the
-  // persistent sb.
-  // startBoundary is a binding variable between betree and journal: we should constrain
-  // our part of sb to garbage collect the log before startBoundary.
-  predicate CommitStart(s: Variables, s': Variables, sb: Superblock, startBoundary: LSN)
-  {
-    && startBoundary <= s.firstValidLSN
-    && SeqsCoveredByAllocation(s, startBoundary, endLSNExclusive(sb.core.firstValidLSN, sb.core.freshestCU), sb.allocation)
-    && sb.core.freshestCU == s.durableTailCU
-    && sb.core.firstValidLSN == startBoundary
-    && s' == s
-  }
-
-  predicate CommitComplete(s: Variables, s': Variables, sb: Superblock)
-  {
-    && s.WF()
-    && s.firstValidLSN <= sb.core.firstValidLSN
-      // guaranteed inductively -- we don't update s.firstValidLSN except here,
-      // CommitStart establishes this relation
-      // and Program carries sb from there to here.
-    && s'.firstValidLSN == sb.core.firstValidLSN
-    && s'.durableTailCU == s.durableTailCU
-    && s'.seqStart == s.seqStart
-    && s'.journal == s.journal
-    && s'.seqToAU == (map seqno | s'.firstValidLSN <= seqno < s'.seqStart :: s.seqToAU[seqno])
+    // Update s'.persistentLSN so that it reflects a persisted LSN (something in the last block,
+    // ideally the last LSN in that block). NB This gives impl freedom to not
+    // record the latest persistent LSN in the freshestCU block, which would be
+    // kind of dumb (it would hold up syncs for no reason), but not unsafe.
+    && (if sb.core.freshestCU.None?
+        then s'.persistentLSN == sb.core.boundaryLSN
+        else 
+          && s'.persistentLSN -1 in s.lsnToCU
+          && s.lsnToCU[s'.persistentLSN - 1] == sb.core.freshestCU.value
+        )
+    && s'.cleanLSN == s.cleanLSN
+    && s'.marshalledLSN == s.marshalledLSN
+    && s'.unmarshalledTail == s.unmarshalledTail
     && s'.syncReqs == s.syncReqs
   }
 
   predicate ReqSync(s: Variables, s': Variables, syncReqId: SyncReqId)
   {
+    && 0 < s.unmarshalledLSN()
     && syncReqId !in s.syncReqs.Keys
-    && s' == s.(syncReqs := s.syncReqs[syncReqId := s.seqStart + |s.journal|])
+    && s' == s.(syncReqs := s.syncReqs[syncReqId := s.unmarshalledLSN()-1])
   }
 
   predicate CompleteSync(s: Variables, s': Variables, syncReqId: SyncReqId)
   {
     && syncReqId in s.syncReqs.Keys
-    && s.syncReqs[syncReqId] < endLSNExclusive(s.firstValidLSN, s.durableTailCU)
+    && s.syncReqs[syncReqId] < s.persistentLSN
     && s' == s.(syncReqs := MapRemove1(s.syncReqs, syncReqId))
   }
-}
 
-module JournalMod {
-  import opened Options
-  import opened Sequences
-  import opened Maps
-  import opened MsgSeqMod
-  import opened AllocationMod
-  import opened JournalMachineMod
+  datatype Step =
+    | AppendStep(message: Message)
+    | AdvanceMarshalledStep(cacheOps: CacheIfc.Ops)
+    | AdvanceCleanStep(cache: CacheIfc.Variables, newClean: nat)
+    | ReallocateStep()
+    | CommitStartStep(cache: CacheIfc.Variables, sb: Superblock, newBoundaryLSN: LSN)
+    | CommitCompleteStep(sb: Superblock)
+    | ReqSyncStep(syncReqId: SyncReqId)
+    | CompleteSyncStep(syncReqId: SyncReqId)
 
-  // Synthesize a superblock that reflects the tail of the chain (cutting
-  // off the first rec), propagating along firstValidLSN.
-  function priorSB(jr:JournalRecord, sb: CoreSuperblock) : CoreSuperblock
-  {
-    CoreSuperblock(jr.priorCU, sb.firstValidLSN)
-  }
-
-  // Monoid-friendly (quantified-list) definition
-  datatype JournalChain = JournalChain(sb: CoreSuperblock, recs:seq<JournalRecord>)
-  {
-    // Synthesize a superblock that reflects the tail of the chain (cutting
-    // off the first rec), propagating along firstValidLSN.
-    function priorSB() : CoreSuperblock
-      requires 0<|recs|
-    {
-      recs[0].priorSB(sb)
+  predicate NextStep(s: Variables, s': Variables, step: Step) {
+    match step {
+      case AppendStep(message) => Append(s, s', message)
+      case AdvanceMarshalledStep(cacheOps) => AdvanceMarshalled(s, s', cacheOps)
+      case AdvanceCleanStep(cache, newClean) => AdvanceClean(s, s', cache, newClean)
+      case ReallocateStep => Reallocate(s, s')
+      case CommitStartStep(cache, sb, newBoundaryLSN) => CommitStart(s, s', cache, sb, newBoundaryLSN)
+      case CommitCompleteStep(sb) => CommitComplete(s, s', sb)
+      case ReqSyncStep(syncReqId) => ReqSync(s, s', syncReqId)
+      case CompleteSyncStep(syncReqId) => CompleteSync(s, s', syncReqId)
     }
   }
 
-  function parse(b: UninterpretedDiskPage) : Option<JournalRecord>
-    // TODO marshalling
-
-  predicate IsLastLink(i: nat, chain: JournalChain)
-    requires 0<=i<|chain.recs|
-  {
-    // stop if nothing more available
-    || chain.recs[i].priorCU.None?
-    // stop if nothing more needed
-    || chain.sb.firstValidLSN >= chain.recs[i].messageSeq.seqStart
-  }
-
-  predicate WFChainBasic(chain: JournalChain)
-  {
-    && (chain.sb.freshestCU.None? <==> 0 == |chain.recs|)
-    && (forall i | 0<=i<|chain.recs| :: i==|chain.recs|-1 <==> IsLastLink(i, chain))
-    && (forall i | 0<=i<|chain.recs|-1 :: chain.recs[i].priorCU.Some?)
-  }
-
-  predicate {:opaque} WFChainInner(chain: JournalChain)
-    requires WFChainBasic(chain)
-  {
-    && (forall i | 0<=i<|chain.recs|-1 ::
-      chain.recs[i].messageSeq.seqStart == chain.recs[i+1].messageSeq.seqEnd)
-  }
-
-  predicate WFChain(chain: JournalChain)
-  {
-    && WFChainBasic(chain)
-    && WFChainInner(chain)
-  }
-
-  function CUsForChain(chain: JournalChain) : (cus: seq<CU>)
-    requires WFChain(chain)
-    ensures |cus| == |chain.recs|
-  {
-    if chain.sb.freshestCU.None?
-    then []
-    else [chain.sb.freshestCU.value] + seq(|chain.recs|-1,
-        i requires 0<=i<|chain.recs|-1 => chain.recs[i].priorCU.value)
-  }
-
-  predicate RecordOnDisk(dv: DiskView, cu: CU, journalRecord: JournalRecord)
-  {
-    && cu in dv
-    && parse(dv[cu]) == Some(journalRecord)
-  }
-
-  predicate {:opaque} ChainMatchesDiskView(dv: DiskView, chain: JournalChain)
-    requires WFChain(chain)
-  {
-    // chain corresponds to stuff in the DiskView starting at freshestCU.
-    && var cus := CUsForChain(chain);
-    && (forall i | 0<=i<|chain.recs| :: RecordOnDisk(dv, cus[i], chain.recs[i]))
-  }
-
-  // Describe a valid chain.
-  predicate ValidJournalChain(dv: DiskView, chain: JournalChain)
-  {
-    && WFChain(chain)
-    && ChainMatchesDiskView(dv, chain)
-  }
-
-  lemma ValidEmptyChain(dv: DiskView, sb: CoreSuperblock)
-    requires sb.freshestCU.None?
-    ensures ValidJournalChain(dv, JournalChain(sb, []))
-  {
-    reveal_WFChainInner();
-    reveal_ChainMatchesDiskView();
-  }
-
-  function ExtendChain(sb: CoreSuperblock, rec: JournalRecord, innerchain: JournalChain)
-    : (chain: JournalChain)
-    requires sb.freshestCU.Some?
-    requires rec.priorCU.Some? ==> sb.firstValidLSN < rec.messageSeq.seqStart; // proves !IsLastLink(0, chain)
-    requires innerchain.sb == rec.priorSB(sb);
-    requires 0<|innerchain.recs| ==> rec.messageSeq.seqStart == innerchain.recs[0].messageSeq.seqEnd;
-    requires WFChain(innerchain)
-    ensures WFChain(chain)
-  {
-    var chain := JournalChain(sb, [rec] + innerchain.recs);
-    assert WFChainBasic(chain) by {
-      forall i | 0<=i<|chain.recs| ensures i==|chain.recs|-1 <==> IsLastLink(i, chain)
-      {
-        if 0<i {
-          assert IsLastLink(i-1, innerchain) == IsLastLink(i, chain);
-        }
-      }
-    }
-    assert WFChainInner(chain) by { reveal_WFChainInner(); }
-    chain
-  }
-
-  // Define reading a chain recursively. Returns None if any of the
-  // CUs point to missing blocks from the dv, or if the block can't
-  // be parsed.
-  // Return the set of readCUs visited. We may read six CUs before returning
-  // a None chain. We have to know that to show how related dvs produce identical
-  // results (even when they're broken).
-  datatype ChainResult = ChainResult(chain: Option<JournalChain>, readCUs:seq<CU>)
-
-  function ChainFrom(dv: DiskView, sb: CoreSuperblock) : (r:ChainResult)
-    ensures r.chain.Some? ==>
-      && ValidJournalChain(dv, r.chain.value)
-      && r.chain.value.sb == sb
-    decreases |dv.Keys|
-  {
-    if sb.freshestCU.None? then
-      // Superblock told the whole story; nothing to read.
-      ValidEmptyChain(dv, sb);
-      ChainResult(Some(JournalChain(sb, [])), [])
-    else if sb.freshestCU.value !in dv then
-      // !RecordOnDisk: tried to read freshestCU and failed
-      ChainResult(None, [sb.freshestCU.value])
-    else
-      var firstRec := parse(dv[sb.freshestCU.value]);
-      if firstRec.None? then
-        // !RecordOnDisk: read freshestCU, but it was borked
-        ChainResult(None, [sb.freshestCU.value])
-      else if firstRec.value.messageSeq.seqEnd <= sb.firstValidLSN then
-        // This isn't an invariant disk state: if we're in the initial call,
-        // the superblock shouldn't point to a useless JournalRecord; if we're
-        // in a recursive call with correctly-chained records, we should have
-        // already ignored this case.
-        ChainResult(None, [sb.freshestCU.value])
-      else if firstRec.value.messageSeq.seqStart == sb.firstValidLSN then
-        // Glad we read this record, but we don't need to read anything beyond.
-        var r := ChainResult(Some(JournalChain(sb, [firstRec.value])), [sb.freshestCU.value]);
-        assert ValidJournalChain(dv, r.chain.value) by {
-          reveal_WFChainInner();
-          reveal_ChainMatchesDiskView();
-        }
-        r
-      else
-        var inner := ChainFrom(MapRemove1(dv, sb.freshestCU.value), firstRec.value.priorSB(sb));
-        if inner.chain.None? // tail didn't decode or
-          // tail decoded but head doesn't stitch to it (a cross-crash invariant)
-          || (0<|inner.chain.value.recs|
-              && firstRec.value.messageSeq.seqStart != inner.chain.value.recs[0].messageSeq.seqEnd)
-        then
-          // failure in recursive call.
-          // We read our cu plus however far the recursive call reached.
-          ChainResult(None, [sb.freshestCU.value] + inner.readCUs)
-        else
-          assert firstRec.value.priorCU.Some? ==> sb.firstValidLSN < firstRec.value.messageSeq.seqStart;
-          var chain := ExtendChain(sb, firstRec.value, inner.chain.value);
-          //var chain := JournalChain(sb, [firstRec.value] + inner.chain.value.recs);
-          assert ValidJournalChain(dv, chain) by {
-            reveal_ChainMatchesDiskView();
-            var cus := CUsForChain(chain);
-            assert forall i | 0<=i<|chain.recs| :: RecordOnDisk(dv, cus[i], chain.recs[i]); // trigger
-          }
-          ChainResult(Some(chain), [sb.freshestCU.value] + inner.readCUs)
-  }
-
-  // TODO redo: return a seq of Message, with a prefix of None.
-  function MessageMaps(journalChain: JournalChain) : seq<MsgSeq> {
-    seq(|journalChain.recs|,
-      i requires 0<=i<|journalChain.recs|
-        => var mm := journalChain.recs[i].messageSeq; mm)
-  }
-
-  // TODO(jonh): collapse to return MsgSeq
-  function IM(dv: DiskView, sb: CoreSuperblock) : seq<MsgSeq>
-  {
-    var chain := ChainFrom(dv, sb).chain;
-    if chain.Some?
-    then
-      MessageMaps(chain.value)
-    else
-      []
-  }
-
-  function ReadAt(cus: seq<CU>, i: nat) : AU
-    requires i<|cus|
-  {
-    cus[i].au
-  }
-
-  // TODO(jonh): Try porting this from recursive style to Travis' suggested
-  // repr-state style (see ReprsAsSets.i.dfy).
-  function IReads(dv: DiskView, sb: CoreSuperblock) : seq<AU>
-  {
-    var cus := ChainFrom(dv, sb).readCUs;
-    // wanted to write:
-    // seq(|cus|, i requires 0<=i<|cus| => cus[i].au)
-    // but Dafny bug, so:
-    seq(|cus|, i requires 0<=i<|cus| => ReadAt(cus, i))
-  }
-
-  predicate SequenceSubset<T>(a:seq<T>, b:seq<T>)
-  {
-    forall i | 0<=i<|a| :: a[i] in b
-  }
-
-  lemma DiskViewsEquivalentAfterRemove(dv0: DiskView, dv1: DiskView, aus: seq<AU>, removedCU: CU, ausr: seq<AU>)
-    requires DiskViewsEquivalentForSet(dv0, dv1, aus)
-    requires SequenceSubset(ausr, aus)
-    ensures DiskViewsEquivalentForSet(MapRemove1(dv0, removedCU), MapRemove1(dv1, removedCU), ausr)
-  {
-  }
-
-  // TODO(jonh): delete chain parameter.
-  lemma FrameOneChain(dv0: DiskView, dv1: DiskView, sb: CoreSuperblock, chain: Option<JournalChain>)
-    requires chain == ChainFrom(dv0, sb).chain
-    requires DiskViewsEquivalentForSet(dv0, dv1, IReads(dv0, sb))
-    ensures chain == ChainFrom(dv1, sb).chain
-    // ensures ChainFrom(dv0, sb).chain == ChainFrom(dv1, sb).chain
-  {
-    if sb.freshestCU.Some? {
-      assert IReads(dv0, sb)[0] == sb.freshestCU.value.au; // trigger
-      if sb.freshestCU.value in dv0 {
-        var firstRec := parse(dv0[sb.freshestCU.value]);
-        if firstRec.Some? { // Recurse to follow chain
-          if firstRec.value.messageSeq.seqEnd <= sb.firstValidLSN {
-          } else if firstRec.value.messageSeq.seqStart == sb.firstValidLSN {
-          } else {
-            var dv0r := MapRemove1(dv0, sb.freshestCU.value);
-            var priorCU := firstRec.value.priorCU;
-            var priorSB := firstRec.value.priorSB(sb);
-            var aus := IReads(dv0, sb);
-            var ausr := if priorCU.Some?
-              then IReads(dv0r, priorSB)
-              else [];
-
-            forall i | 0<=i<|ausr| ensures ausr[i] in aus {
-              assert aus[i+1] == ausr[i]; // witness to SequenceSubset(ausr, aus)
-            }
-            DiskViewsEquivalentAfterRemove(dv0, dv1, aus, sb.freshestCU.value, ausr);
-            FrameOneChain(dv0r, MapRemove1(dv1, sb.freshestCU.value),
-              priorSB, ChainFrom(dv0r, priorSB).chain);
-          }
-        }
-      }
-    }
-  }
-
-  lemma Framing(sb:CoreSuperblock, dv0: DiskView, dv1: DiskView)
-    requires DiskViewsEquivalentForSet(dv0, dv1, IReads(dv0, sb))
-    ensures IM(dv0, sb) == IM(dv1, sb)
-  {
-    FrameOneChain(dv0, dv1, sb, ChainFrom(dv0, sb).chain);
+  predicate Next(s: Variables, s': Variables) {
+    exists step :: NextStep(s, s', step)
   }
 }
