Splinter/JournalInterp.i.dfy
@@ -1,0 +1,270 @@
+include "Journal.i.dfy"
+
+module JournalMod {
+  import opened Options
+  import opened Sequences
+  import opened Maps
+  import opened MsgSeqMod
+  import opened AllocationMod
+  import opened JournalMachineMod
+
+  // Synthesize a superblock that reflects the tail of the chain (cutting
+  // off the first rec), propagating along boundaryLSN.
+  function priorSB(jr:JournalRecord, sb: CoreSuperblock) : CoreSuperblock
+  {
+    CoreSuperblock(jr.priorCU, sb.boundaryLSN)
+  }
+
+  // Monoid-friendly (quantified-list) definition
+  datatype JournalChain = JournalChain(sb: CoreSuperblock, recs:seq<JournalRecord>)
+  {
+    // Synthesize a superblock that reflects the tail of the chain (cutting
+    // off the first rec), propagating along boundaryLSN.
+    function priorSB() : CoreSuperblock
+      requires 0<|recs|
+    {
+      recs[0].priorSB(sb)
+    }
+  }
+
+  predicate IsLastLink(i: nat, chain: JournalChain)
+    requires 0<=i<|chain.recs|
+  {
+    // stop if nothing more available
+    || chain.recs[i].priorCU.None?
+    // stop if nothing more needed
+    || chain.sb.boundaryLSN >= chain.recs[i].messageSeq.seqStart
+  }
+
+  predicate WFChainBasic(chain: JournalChain)
+  {
+    && (chain.sb.freshestCU.None? <==> 0 == |chain.recs|)
+    && (forall i | 0<=i<|chain.recs| :: i==|chain.recs|-1 <==> IsLastLink(i, chain))
+    && (forall i | 0<=i<|chain.recs|-1 :: chain.recs[i].priorCU.Some?)
+  }
+
+  predicate {:opaque} WFChainInner(chain: JournalChain)
+    requires WFChainBasic(chain)
+  {
+    && (forall i | 0<=i<|chain.recs|-1 ::
+      chain.recs[i].messageSeq.seqStart == chain.recs[i+1].messageSeq.seqEnd)
+  }
+
+  predicate WFChain(chain: JournalChain)
+  {
+    && WFChainBasic(chain)
+    && WFChainInner(chain)
+  }
+
+  function CUsForChain(chain: JournalChain) : (cus: seq<CU>)
+    requires WFChain(chain)
+    ensures |cus| == |chain.recs|
+  {
+    if chain.sb.freshestCU.None?
+    then []
+    else [chain.sb.freshestCU.value] + seq(|chain.recs|-1,
+        i requires 0<=i<|chain.recs|-1 => chain.recs[i].priorCU.value)
+  }
+
+  predicate RecordOnDisk(dv: DiskView, cu: CU, journalRecord: JournalRecord)
+  {
+    && cu in dv
+    && parse(dv[cu]) == Some(journalRecord)
+  }
+
+  predicate {:opaque} ChainMatchesDiskView(dv: DiskView, chain: JournalChain)
+    requires WFChain(chain)
+  {
+    // chain corresponds to stuff in the DiskView starting at freshestCU.
+    && var cus := CUsForChain(chain);
+    && (forall i | 0<=i<|chain.recs| :: RecordOnDisk(dv, cus[i], chain.recs[i]))
+  }
+
+  // Describe a valid chain.
+  predicate ValidJournalChain(dv: DiskView, chain: JournalChain)
+  {
+    && WFChain(chain)
+    && ChainMatchesDiskView(dv, chain)
+  }
+
+  lemma ValidEmptyChain(dv: DiskView, sb: CoreSuperblock)
+    requires sb.freshestCU.None?
+    ensures ValidJournalChain(dv, JournalChain(sb, []))
+  {
+    reveal_WFChainInner();
+    reveal_ChainMatchesDiskView();
+  }
+
+  function ExtendChain(sb: CoreSuperblock, rec: JournalRecord, innerchain: JournalChain)
+    : (chain: JournalChain)
+    requires sb.freshestCU.Some?
+    requires rec.priorCU.Some? ==> sb.boundaryLSN < rec.messageSeq.seqStart; // proves !IsLastLink(0, chain)
+    requires innerchain.sb == rec.priorSB(sb);
+    requires 0<|innerchain.recs| ==> rec.messageSeq.seqStart == innerchain.recs[0].messageSeq.seqEnd;
+    requires WFChain(innerchain)
+    ensures WFChain(chain)
+  {
+    var chain := JournalChain(sb, [rec] + innerchain.recs);
+    assert WFChainBasic(chain) by {
+      forall i | 0<=i<|chain.recs| ensures i==|chain.recs|-1 <==> IsLastLink(i, chain)
+      {
+        if 0<i {
+          assert IsLastLink(i-1, innerchain) == IsLastLink(i, chain);
+        }
+      }
+    }
+    assert WFChainInner(chain) by { reveal_WFChainInner(); }
+    chain
+  }
+
+  // Define reading a chain recursively. Returns None if any of the
+  // CUs point to missing blocks from the dv, or if the block can't
+  // be parsed.
+  // Return the set of readCUs visited. We may read six CUs before returning
+  // a None chain. We have to know that to show how related dvs produce identical
+  // results (even when they're broken).
+  datatype ChainResult = ChainResult(chain: Option<JournalChain>, readCUs:seq<CU>)
+
+  function ChainFrom(dv: DiskView, sb: CoreSuperblock) : (r:ChainResult)
+    ensures r.chain.Some? ==>
+      && ValidJournalChain(dv, r.chain.value)
+      && r.chain.value.sb == sb
+    decreases |dv.Keys|
+  {
+    if sb.freshestCU.None? then
+      // Superblock told the whole story; nothing to read.
+      ValidEmptyChain(dv, sb);
+      ChainResult(Some(JournalChain(sb, [])), [])
+    else if sb.freshestCU.value !in dv then
+      // !RecordOnDisk: tried to read freshestCU and failed
+      ChainResult(None, [sb.freshestCU.value])
+    else
+      var firstRec := parse(dv[sb.freshestCU.value]);
+      if firstRec.None? then
+        // !RecordOnDisk: read freshestCU, but it was borked
+        ChainResult(None, [sb.freshestCU.value])
+      else if firstRec.value.messageSeq.seqEnd <= sb.boundaryLSN then
+        // This isn't an invariant disk state: if we're in the initial call,
+        // the superblock shouldn't point to a useless JournalRecord; if we're
+        // in a recursive call with correctly-chained records, we should have
+        // already ignored this case.
+        ChainResult(None, [sb.freshestCU.value])
+      else if firstRec.value.messageSeq.seqStart == sb.boundaryLSN then
+        // Glad we read this record, but we don't need to read anything beyond.
+        var r := ChainResult(Some(JournalChain(sb, [firstRec.value])), [sb.freshestCU.value]);
+        assert ValidJournalChain(dv, r.chain.value) by {
+          reveal_WFChainInner();
+          reveal_ChainMatchesDiskView();
+        }
+        r
+      else
+        var inner := ChainFrom(MapRemove1(dv, sb.freshestCU.value), firstRec.value.priorSB(sb));
+        if inner.chain.None? // tail didn't decode or
+          // tail decoded but head doesn't stitch to it (a cross-crash invariant)
+          || (0<|inner.chain.value.recs|
+              && firstRec.value.messageSeq.seqStart != inner.chain.value.recs[0].messageSeq.seqEnd)
+        then
+          // failure in recursive call.
+          // We read our cu plus however far the recursive call reached.
+          ChainResult(None, [sb.freshestCU.value] + inner.readCUs)
+        else
+          assert firstRec.value.priorCU.Some? ==> sb.boundaryLSN < firstRec.value.messageSeq.seqStart;
+          var chain := ExtendChain(sb, firstRec.value, inner.chain.value);
+          //var chain := JournalChain(sb, [firstRec.value] + inner.chain.value.recs);
+          assert ValidJournalChain(dv, chain) by {
+            reveal_ChainMatchesDiskView();
+            var cus := CUsForChain(chain);
+            assert forall i | 0<=i<|chain.recs| :: RecordOnDisk(dv, cus[i], chain.recs[i]); // trigger
+          }
+          ChainResult(Some(chain), [sb.freshestCU.value] + inner.readCUs)
+  }
+
+  // TODO redo: return a seq of Message, with a prefix of None.
+  function MessageMaps(journalChain: JournalChain) : seq<MsgSeq> {
+    seq(|journalChain.recs|,
+      i requires 0<=i<|journalChain.recs|
+        => var mm := journalChain.recs[i].messageSeq; mm)
+  }
+
+  // TODO(jonh): collapse to return MsgSeq
+  function IM(dv: DiskView, sb: CoreSuperblock) : seq<MsgSeq>
+  {
+    var chain := ChainFrom(dv, sb).chain;
+    if chain.Some?
+    then
+      MessageMaps(chain.value)
+    else
+      []
+  }
+
+  function ReadAt(cus: seq<CU>, i: nat) : AU
+    requires i<|cus|
+  {
+    cus[i].au
+  }
+
+  // TODO(jonh): Try porting this from recursive style to Travis' suggested
+  // repr-state style (see ReprsAsSets.i.dfy).
+  function IReads(dv: DiskView, sb: CoreSuperblock) : seq<AU>
+  {
+    var cus := ChainFrom(dv, sb).readCUs;
+    // wanted to write:
+    // seq(|cus|, i requires 0<=i<|cus| => cus[i].au)
+    // but Dafny bug, so:
+    seq(|cus|, i requires 0<=i<|cus| => ReadAt(cus, i))
+  }
+
+  predicate SequenceSubset<T>(a:seq<T>, b:seq<T>)
+  {
+    forall i | 0<=i<|a| :: a[i] in b
+  }
+
+  lemma DiskViewsEquivalentAfterRemove(dv0: DiskView, dv1: DiskView, aus: seq<AU>, removedCU: CU, ausr: seq<AU>)
+    requires DiskViewsEquivalentForSet(dv0, dv1, aus)
+    requires SequenceSubset(ausr, aus)
+    ensures DiskViewsEquivalentForSet(MapRemove1(dv0, removedCU), MapRemove1(dv1, removedCU), ausr)
+  {
+  }
+
+  // TODO(jonh): delete chain parameter.
+  lemma FrameOneChain(dv0: DiskView, dv1: DiskView, sb: CoreSuperblock, chain: Option<JournalChain>)
+    requires chain == ChainFrom(dv0, sb).chain
+    requires DiskViewsEquivalentForSet(dv0, dv1, IReads(dv0, sb))
+    ensures chain == ChainFrom(dv1, sb).chain
+    // ensures ChainFrom(dv0, sb).chain == ChainFrom(dv1, sb).chain
+  {
+    if sb.freshestCU.Some? {
+      assert IReads(dv0, sb)[0] == sb.freshestCU.value.au; // trigger
+      if sb.freshestCU.value in dv0 {
+        var firstRec := parse(dv0[sb.freshestCU.value]);
+        if firstRec.Some? { // Recurse to follow chain
+          if firstRec.value.messageSeq.seqEnd <= sb.boundaryLSN {
+          } else if firstRec.value.messageSeq.seqStart == sb.boundaryLSN {
+          } else {
+            var dv0r := MapRemove1(dv0, sb.freshestCU.value);
+            var priorCU := firstRec.value.priorCU;
+            var priorSB := firstRec.value.priorSB(sb);
+            var aus := IReads(dv0, sb);
+            var ausr := if priorCU.Some?
+              then IReads(dv0r, priorSB)
+              else [];
+
+            forall i | 0<=i<|ausr| ensures ausr[i] in aus {
+              assert aus[i+1] == ausr[i]; // witness to SequenceSubset(ausr, aus)
+            }
+            DiskViewsEquivalentAfterRemove(dv0, dv1, aus, sb.freshestCU.value, ausr);
+            FrameOneChain(dv0r, MapRemove1(dv1, sb.freshestCU.value),
+              priorSB, ChainFrom(dv0r, priorSB).chain);
+          }
+        }
+      }
+    }
+  }
+
+  lemma Framing(sb:CoreSuperblock, dv0: DiskView, dv1: DiskView)
+    requires DiskViewsEquivalentForSet(dv0, dv1, IReads(dv0, sb))
+    ensures IM(dv0, sb) == IM(dv1, sb)
+  {
+    FrameOneChain(dv0, dv1, sb, ChainFrom(dv0, sb).chain);
+  }
+}
